First attempt at external validity of lists

src/Utils.dfy
@@ -3,16 +3,37 @@ function method BigUnion<A>(S: set<set<A>>): set<A>
   set X, x | X in S && x in X :: x
 }
 
-function method elems<A>(l: array<A>): set<A>
-  reads l
-{
-  set x | x in l[..]
+module Array {
+  function method elems<A>(l: array<A>): set<A>
+    reads l
+  {
+    set x | x in l[..]
+  }
 }
 
-function rev<A>(xs: seq<A>): seq<A>
-{
-  if |xs| == 0 then
-    []
-  else
-    rev(xs[1..]) + [xs[0]]
+module Seq {
+  function Rev<A>(xs: seq<A>): seq<A>
+  {
+    if |xs| == 0 then
+      []
+    else
+      Rev(xs[1..]) + [xs[0]]
+  }
+
+  function Map<A,B>(f: A -> B, xs: seq<A>): seq<B>
+  {
+    if xs == [] then
+      []
+    else
+      [f(xs[0])] + Map(f, xs[1..])
+  }
+
+  function Elems<A>(xs: seq<A>): set<A>
+  {
+    set x | x in xs
+  }
+
+  lemma InEquivInMultiset<A>(xs: seq<A>)
+    ensures forall x :: x in xs <==> x in multiset(xs)
+  {}
 }
