src/ListSeq.dfy
@@ -1,0 +1,203 @@
+include "Utils.dfy"
+
+class Node<A> {
+  var data: A;
+  var next: Node?<A>;
+
+  constructor(data: A, next: Node?<A>)
+    ensures this.data == data
+    ensures this.next == next
+  {
+    this.data := data;
+    this.next := next;
+  }
+
+  predicate IsPrevOf(n: Node<A>)
+    reads this
+  {
+    next == n
+  }
+}
+
+class List<A> {
+  var head: Node?<A>;
+  var spine: seq<Node<A>>;
+
+  predicate Valid()
+    reads this, spine
+  {
+    && (forall i | 0 <= i < |spine|-1 :: spine[i].IsPrevOf(spine[i+1]))
+    && (if head == null then
+        spine == []
+      else
+        spine != [] && spine[0] == head && spine[|spine|-1].next == null
+      )
+  }
+
+  lemma HeadInSpine()
+    requires Valid()
+    ensures head != null ==> head in spine
+  {
+  }
+
+  static function ModelAux(xs: seq<Node<A>>): seq<A>
+    reads multiset(xs)
+  {
+    if xs == [] then
+      []
+    else
+      [xs[0].data] + ModelAux(xs[1..])
+  }
+
+  function Model(): seq<A>
+    reads this, spine, multiset(spine)
+    requires Valid()
+  {
+    ModelAux(spine)
+  }
+
+  constructor()
+    ensures Valid()
+    ensures Model() == []
+  {
+    head := null;
+    spine := [];
+  }
+
+  method Pop() returns (res: A)
+    modifies this
+    requires head != null
+    requires Valid()
+    ensures Valid()
+    ensures res == old(head.data)
+    ensures [res] + Model() == old(Model())
+    ensures [old(head)] + spine == old(spine)
+  {
+    res := head.data;
+    if head.next == null {
+      if |spine| != 1 {
+        assert |spine| >= 2;
+        assert spine[0].next == spine[1];
+        assert false;
+      } else {
+        assert spine == [head];
+      }
+      assert spine == [head];
+    }
+    head := head.next;
+    spine := spine[1..];
+    if head == null {
+      assert spine == [];
+    }
+  }
+
+  method Push(x: A)
+    modifies this
+    requires Valid()
+    ensures Valid()
+    ensures Model() == [x] + old(Model())
+    ensures spine == [head] + old(spine)
+    ensures fresh(Seq.Elems(spine) - old(Seq.Elems(spine)))
+    ensures fresh(Seq.Elems(spine) - Seq.Elems(old(spine)))
+    // ensures fresh(multiset(spine) - old(multiset(spine)))
+    ensures fresh(head)
+  {
+    head := new Node(x, head);
+    spine := [head] + spine;
+  }
+
+  method Append(other: List<A>)
+    decreases spine
+    modifies this
+    requires Valid()
+    requires other.Valid()
+    // At first I didn't add the next precondition. In a language without
+    // verification like C maybe I would have forgotten about it, but the function
+    // doesn't work the way you expect it to if you don't keep this precondition
+    // in mind. This could have resulted in segmentation faults or buggy code.
+    // Another win for formal verification!
+    requires this != other
+    ensures Valid()
+    ensures Model() == old(Model()) + other.Model()
+  {
+    if head == null {
+      head := other.head;
+      spine := other.spine;
+    } else {
+      var x := Pop();
+      Append(other);
+      Push(x);
+    }
+  }
+
+  method PopPush(other: List<A>)
+    modifies this, other
+    requires head != null
+    requires Valid()
+    requires other.Valid()
+    requires multiset(spine) !! multiset(other.spine)
+    ensures multiset(spine) !! multiset(other.spine)
+    ensures Valid()
+    ensures other.Valid()
+    // ensures Seq.Rev(old(spine)) + old(other.spine) == Seq.Rev(spine) + other.spine
+    ensures old(multiset(spine)) > multiset(spine)
+    ensures Seq.Rev(old(Model())) + old(other.Model())
+      == Seq.Rev(Model()) + other.Model()
+  {
+    ghost var ospine := spine;
+    ghost var ootherspine := other.spine;
+    ghost var ohead := head;
+    assert multiset(spine) !! multiset(other.spine);
+    other.HeadInSpine();
+    assert head in spine;
+    if other.head == null {
+      assert this != other;
+    } else {
+      assert other.head in other.spine;
+      assert multiset(spine) !! multiset(other.spine);
+      // assert forall x :: x in multiset(spine) ==> x !in multiset(other.spine);
+      assert forall x :: x in multiset(spine) <== x !in multiset(other.spine);
+      assert forall x :: x in multiset(spine) <==> x !in multiset(other.spine);
+      assert forall xs: seq<A>, x: A :: x in xs <==> x in multiset(xs);
+      Seq.InEquivInMultiset(spine);
+      assert forall x :: x in spine <==> x in multiset(spine);
+      assert forall x :: x in other.spine <==> x in multiset(other.spine);
+      assert forall x :: x in spine <== x !in other.spine;
+      assert head != other.head;
+      assert this != other;
+    }
+    assert this != other;
+    assert multiset(spine) !! multiset(other.spine);
+    assert this != other;
+    var x := Pop();
+    assert this != other;
+    assert multiset(spine) !! multiset(other.spine);
+    assert this != other;
+    other.Push(x);
+    assert this != other;
+    assert multiset(spine) !! multiset(other.spine);
+  }
+
+  method Reverse()
+    modifies this
+    requires Valid()
+    ensures Valid()
+    ensures Model() == Seq.Rev(old(Model()))
+  {
+    ghost var omodel := Model();
+    var aux := new List();
+    aux.head := head;
+    aux.spine := spine;
+    head := null;
+    spine := [];
+    while aux.head != null
+      decreases multiset(aux.spine)
+      invariant Valid()
+      invariant aux.Valid()
+      invariant Seq.Rev(omodel) == Seq.Rev(aux.Model()) + Model()
+      invariant multiset(spine) !! multiset(aux.spine);
+    {
+      aux.PopPush(this);
+    }
+  }
+}
